theories/lang/cpp/compile.v
@@ -25,22 +25,22 @@ Section with_Σ.
       compiled code ([fspec]).
    *)
   Axiom code_at_ok : forall (f : Func) p,
-      code_at f p
+      code_at σ f p
       |-- Forall ti ls Q, wp_func (resolve:=σ) f ti ls Q -*
                           fspec (Σ:=Σ) σ.(genv_tu).(globals) (type_of_value (Ofunction f)) ti (Vptr p) ls Q.
 
   Axiom method_at_ok : forall (m : Method) p,
-      method_at m p
+      method_at σ m p
       |-- Forall ti ls Q, wp_method (resolve:=σ) m ti ls Q -*
                           fspec (Σ:=Σ) σ.(genv_tu).(globals) (type_of_value (Omethod m)) ti (Vptr p) ls Q.
 
   Axiom ctor_at_ok : forall (c : Ctor) p,
-      ctor_at c p
+      ctor_at σ c p
       |-- Forall ti ls Q, wp_ctor (resolve:=σ) c ti ls Q -*
                           fspec σ.(genv_tu).(globals) (type_of_value (Oconstructor c)) ti (Vptr p) ls Q.
 
   Axiom dtor_at_ok : forall (d : Dtor) p,
-      dtor_at d p
+      dtor_at σ d p
       |-- Forall ti ls Q, wp_dtor (resolve:=σ) d ti ls Q -*
                           fspec σ.(genv_tu).(globals) (type_of_value (Odestructor d)) ti (Vptr p) ls Q.
 
